Merge iAssert and iPvsAssert.
To do so, we have introduced the specialization patterns:

  =>[H1 .. Hn] and =>[-H1 .. Hn]

That generate a goal in which the view shift is preserved. These specialization
patterns can also be used for e.g. iApply.

Note that this machinery is not tied to primitive view shifts, and works for
various kinds of goal (as captured by the ToAssert type class, which describes
how to transform the asserted goal based on the main goal).

TODO: change the name of these specialization patterns to reflect this
generality.

proofmode/coq_tactics.v
@@ -494,24 +494,28 @@ Proof.
     by rewrite right_id assoc (to_wand R) always_if_elim wand_elim_r wand_elim_r.
 Qed.
 
-Lemma tac_specialize_assert Δ Δ' Δ1 Δ2' j q lr js P1 P2 R Q :
+Class ToAssert (P : uPred M) (Q : uPred M) (R : uPred M) :=
+  to_assert : (R ★ (P -★ Q)) ⊢ Q.
+Global Arguments to_assert _ _ _ {_}.
+Lemma to_assert_fallthrough P Q : ToAssert P Q P.
+Proof. by rewrite /ToAssert wand_elim_r. Qed.
+
+Lemma tac_specialize_assert Δ Δ' Δ1 Δ2' j q lr js R P1 P2 P1' Q :
   envs_lookup_delete j Δ = Some (q, R, Δ') →
-  ToWand R P1 P2 →
+  ToWand R P1 P2 → ToAssert P1 Q P1' →
   ('(Δ1,Δ2) ← envs_split lr js Δ';
-    Δ2' ← envs_app (envs_persistent Δ1 && q) (Esnoc Enil j P2) Δ2;
+    Δ2' ← envs_app false (Esnoc Enil j P2) Δ2;
     Some (Δ1,Δ2')) = Some (Δ1,Δ2') → (* does not preserve position of [j] *)
-  Δ1 ⊢ P1 → Δ2' ⊢ Q → Δ ⊢ Q.
+  Δ1 ⊢ P1' → Δ2' ⊢ Q → Δ ⊢ Q.
 Proof.
-  intros [? ->]%envs_lookup_delete_Some ?? HP1 <-.
+  intros [? ->]%envs_lookup_delete_Some ??? HP1 HQ.
   destruct (envs_split _ _ _) as [[? Δ2]|] eqn:?; simplify_eq/=;
     destruct (envs_app _ _ _) eqn:?; simplify_eq/=.
   rewrite envs_lookup_sound // envs_split_sound //.
   rewrite (envs_app_sound Δ2) //; simpl.
-  destruct (envs_persistent Δ1) eqn:?; simplify_eq/=.
-  - rewrite right_id (to_wand R) (persistentP Δ1) HP1.
-    by rewrite assoc (always_elim_if q) -always_if_sep wand_elim_l wand_elim_r.
-  - rewrite right_id (to_wand R).
-    by rewrite always_if_elim assoc HP1 wand_elim_l wand_elim_r.
+  rewrite right_id (to_wand R) HP1 assoc -(comm _ P1') -assoc.
+  rewrite -(to_assert P1 Q); apply sep_mono_r, wand_intro_l.
+  by rewrite always_if_elim assoc !wand_elim_r.
 Qed.
 
 Lemma tac_specialize_pure Δ Δ' j q R P1 P2 φ Q :
@@ -559,14 +563,15 @@ Proof.
   intros HΔ. by rewrite envs_clear_spatial_sound HΔ env_fold_wand wand_elim_l.
 Qed.
 
-Lemma tac_assert Δ Δ1 Δ2 Δ2' lr js j P Q :
+Lemma tac_assert Δ Δ1 Δ2 Δ2' lr js j P Q R :
+  ToAssert P Q R →
   envs_split lr js Δ = Some (Δ1,Δ2) →
   envs_app false (Esnoc Enil j P) Δ2 = Some Δ2' →
-  Δ1 ⊢ P → Δ2' ⊢ Q → Δ ⊢ Q.
+  Δ1 ⊢ R → Δ2' ⊢ Q → Δ ⊢ Q.
 Proof.
-  intros ?? HP HQ. rewrite envs_split_sound //.
+  intros ??? HP HQ. rewrite envs_split_sound //.
   rewrite (envs_app_sound Δ2) //; simpl.
-  by rewrite right_id HP HQ wand_elim_r.
+  by rewrite right_id HP HQ.
 Qed.
 
 Lemma tac_assert_persistent Δ Δ' j P Q :
